coq/NNRSimp/Lang/NNRSimpVars.v
@@ -16,6 +16,7 @@
 
 Require Import String.
 Require Import List.
+Require Import Permutation.
 Require Import Arith.
 Require Import EquivDec.
 Require Import Morphisms.
@@ -25,6 +26,7 @@ Require Import Bool.
 Require Import Peano_dec.
 Require Import EquivDec.
 Require Import Decidable.
+
 Require Import Utils.
 Require Import CommonRuntime.
 Require Import NNRSimp.
@@ -80,5 +82,120 @@ Section NNRSimpVars.
        | NNRSimpEither e x₁ s₁ x₂ s₂ =>
          x₁::(nnrs_imp_stmt_bound_vars s₁) ++ x₂::(nnrs_imp_stmt_bound_vars s₂)
        end.
+
+  Fixpoint nnrs_imp_stmt_mayberead_vars (s:nnrs_imp_stmt) : list var
+    := match s with
+       | NNRSimpSkip => nil
+       | NNRSimpSeq s₁ s₂ =>
+         nnrs_imp_stmt_mayberead_vars s₁ ++ nnrs_imp_stmt_mayberead_vars s₂
+       | NNRSimpAssign v e =>
+         nnrs_imp_expr_free_vars e
+       | NNRSimpLet v eo s₀ =>
+         match eo with
+         | Some e => nnrs_imp_expr_free_vars e
+         | None => nil
+         end ++ remove string_eqdec v (nnrs_imp_stmt_mayberead_vars s₀)
+       | NNRSimpFor v e s₀ =>
+         nnrs_imp_expr_free_vars e ++ remove string_eqdec v (nnrs_imp_stmt_mayberead_vars s₀)
+       | NNRSimpIf e s₁ s₂ =>
+         nnrs_imp_expr_free_vars e ++ nnrs_imp_stmt_mayberead_vars s₁ ++ nnrs_imp_stmt_mayberead_vars s₂
+       | NNRSimpEither e x₁ s₁ x₂ s₂ =>
+         nnrs_imp_expr_free_vars e ++ remove string_eqdec x₁ (nnrs_imp_stmt_mayberead_vars s₁) ++ remove string_eqdec x₂ (nnrs_imp_stmt_mayberead_vars s₂)
+       end.
+
+    Fixpoint nnrs_imp_stmt_maybewritten_vars (s:nnrs_imp_stmt) : list var
+    := match s with
+       | NNRSimpSkip => nil
+       | NNRSimpSeq s₁ s₂ =>
+         nnrs_imp_stmt_maybewritten_vars s₁ ++ nnrs_imp_stmt_maybewritten_vars s₂
+       | NNRSimpAssign v e =>
+         v::nil
+       | NNRSimpLet v eo s₀ =>
+         remove string_eqdec v (nnrs_imp_stmt_maybewritten_vars s₀)
+       | NNRSimpFor v e s₀ =>
+         remove string_eqdec v (nnrs_imp_stmt_maybewritten_vars s₀)
+       | NNRSimpIf e s₁ s₂ =>
+         nnrs_imp_stmt_maybewritten_vars s₁ ++ nnrs_imp_stmt_maybewritten_vars s₂
+       | NNRSimpEither e x₁ s₁ x₂ s₂ =>
+         remove string_eqdec x₁ (nnrs_imp_stmt_maybewritten_vars s₁) ++ remove string_eqdec x₂ (nnrs_imp_stmt_maybewritten_vars s₂)
+       end.
+
+    Global Instance remove_perm_proper {A} dec v :
+      Proper ((@Permutation A) ==> (@Permutation A)) (remove dec v).
+    Proof.
+      unfold Proper, respectful.
+      apply Permutation_ind_bis; simpl; intros.
+      - trivial.
+      - match_destr.
+        eauto.
+      - repeat match_destr; eauto.
+        rewrite H0.
+        apply perm_swap.
+      - etransitivity; eauto.
+    Qed.
+        
+    Lemma nnrs_imp_stmt_free_vars_readwrite_perm (s:nnrs_imp_stmt)
+      : Permutation
+          (nnrs_imp_stmt_free_vars s)
+          (nnrs_imp_stmt_mayberead_vars s ++ nnrs_imp_stmt_maybewritten_vars s).
+    Proof.
+      nnrs_imp_stmt_cases (induction s) Case
+      ; simpl.
+      - Case "NNRSimpSkip"%string.
+        trivial.
+      - Case "NNRSimpSeq"%string.
+        rewrite IHs1, IHs2.
+        repeat rewrite app_ass.
+        apply Permutation_app; try reflexivity.
+        repeat rewrite <- app_ass.
+        apply Permutation_app; try reflexivity.
+        apply Permutation_app_swap.
+      - Case "NNRSimpAssign"%string.
+        apply Permutation_cons_append.
+      - Case "NNRSimpLet"%string.
+        rewrite app_ass.
+        apply Permutation_app; try reflexivity.
+        rewrite list_remove_append_distrib.
+        apply remove_perm_proper; trivial.
+      - Case "NNRSimpFor"%string.
+        rewrite app_ass.
+        apply Permutation_app; try reflexivity.
+        rewrite list_remove_append_distrib.
+        apply remove_perm_proper; trivial.
+      - Case "NNRSimpIf"%string.
+        rewrite app_ass.
+        apply Permutation_app; try reflexivity.
+        rewrite IHs1, IHs2.
+        repeat rewrite app_ass.
+        apply Permutation_app; try reflexivity.
+        repeat rewrite <- app_ass.
+        apply Permutation_app; try reflexivity.
+        apply Permutation_app_swap.
+      - Case "NNRSimpEither"%string.
+        rewrite app_ass.
+        apply Permutation_app; try reflexivity.
+        transitivity (
+            ((remove string_eqdec v (nnrs_imp_stmt_mayberead_vars s1))
+                     ++ remove string_eqdec v (nnrs_imp_stmt_maybewritten_vars s1))
+               ++
+               ((remove string_eqdec v0 (nnrs_imp_stmt_mayberead_vars s2))
+                  ++ remove string_eqdec v0 (nnrs_imp_stmt_maybewritten_vars s2))).
+        + repeat rewrite list_remove_append_distrib.
+          apply Permutation_app
+          ; apply remove_perm_proper; trivial.
+        + repeat rewrite app_ass.
+          apply Permutation_app; try reflexivity.
+          repeat rewrite <- app_ass.
+          apply Permutation_app; try reflexivity.
+          apply Permutation_app_swap.
+    Qed.
+
+    Lemma nnrs_imp_stmt_free_vars_readwrite_equiv (s:nnrs_imp_stmt)
+      : equivlist
+          (nnrs_imp_stmt_free_vars s)
+          (nnrs_imp_stmt_mayberead_vars s ++ nnrs_imp_stmt_maybewritten_vars s).
+    Proof.
+      rewrite nnrs_imp_stmt_free_vars_readwrite_perm; reflexivity.
+    Qed.
 
 End NNRSimpVars.
