coq/NNRSimp/Optim/NNRSimpRewrite.v
@@ -47,5 +47,1164 @@ Section NNRSimpRewrite.
     red; simpl; trivial.
   Qed.
 
+  (* renaming *)
+  Lemma rename_let_eq x x' e s:
+    ~ In x' (nnrs_imp_stmt_free_vars s) ->
+    ~ In x' (nnrs_imp_stmt_bound_vars s) ->
+    (NNRSimpLet x e s) ≡ˢ
+            (NNRSimpLet x' e (nnrs_imp_stmt_rename s x x')).
+  Proof.
+    intros nin1 nin2.
+    red; simpl; intros.
+    destruct e; simpl; trivial.
+    - apply olift_ext; intros.
+      generalize (nnrs_imp_stmt_eval_rename h σc σ s x x' a nin1 nin2)
+      ; intros HH.
+      unfold var in *.
+      repeat match_option_in HH
+      ; repeat match_destr_in HH
+      ; try contradiction.
+      intuition congruence.
+    - generalize (nnrs_imp_stmt_eval_rename h σc σ s x x' None nin1 nin2)
+      ; intros HH.
+      unfold var in *.
+      repeat match_option_in HH
+      ; repeat match_destr_in HH
+      ; try contradiction.
+      intuition congruence.
+  Qed.
+
+  Lemma rename_for_eq x x' e s:
+    ~ In x' (nnrs_imp_stmt_free_vars s) ->
+    ~ In x' (nnrs_imp_stmt_bound_vars s) ->
+    (NNRSimpFor x e s) ≡ˢ
+            (NNRSimpFor x' e (nnrs_imp_stmt_rename s x x')).
+  Proof.
+    intros nin1 nin2.
+    red; simpl; intros.
+    match_destr.
+    destruct d; simpl; trivial.
+    clear dn_σ e.
+    revert σ.
+    induction l; simpl; trivial; intros σ.
+      generalize (nnrs_imp_stmt_eval_rename h σc σ s x x' (Some a) nin1 nin2)
+      ; intros HH.
+      unfold var in *.
+      repeat match_option_in HH
+      ; repeat match_destr_in HH
+      ; try contradiction.
+      intuition congruence.
+  Qed.
+
+  Lemma rename_either_l_eq e s₁ x₁ x₁' x₂ s₂:
+    ~ In x₁' (nnrs_imp_stmt_free_vars s₁) ->
+    ~ In x₁' (nnrs_imp_stmt_bound_vars s₁) ->
+    (NNRSimpEither e x₁ s₁ x₂ s₂) ≡ˢ
+            (NNRSimpEither e x₁' (nnrs_imp_stmt_rename s₁ x₁ x₁') x₂ s₂).
+  Proof.
+    intros nin1 nin2.
+    red; simpl; intros.
+    match_destr.
+    destruct d; simpl; trivial.
+    generalize (nnrs_imp_stmt_eval_rename h σc σ s₁ x₁ x₁' (Some d) nin1 nin2)
+    ; intros HH.
+    unfold var in *.
+    repeat match_option_in HH
+    ; repeat match_destr_in HH
+    ; try contradiction.
+    intuition congruence.
+  Qed.
+
+  Lemma rename_either_r_eq e s₁ x₁ x₂ x₂'  s₂:
+    ~ In x₂' (nnrs_imp_stmt_free_vars s₂) ->
+    ~ In x₂' (nnrs_imp_stmt_bound_vars s₂) ->
+    (NNRSimpEither e x₁ s₁ x₂ s₂) ≡ˢ
+            (NNRSimpEither e x₁ s₁ x₂' (nnrs_imp_stmt_rename s₂ x₂ x₂')).
+  Proof.
+    intros nin1 nin2.
+    red; simpl; intros.
+    match_destr.
+    destruct d; simpl; trivial.
+    generalize (nnrs_imp_stmt_eval_rename h σc σ s₂ x₂ x₂' (Some d) nin1 nin2)
+    ; intros HH.
+    unfold var in *.
+    repeat match_option_in HH
+    ; repeat match_destr_in HH
+    ; try contradiction.
+    intuition congruence.
+  Qed.
+    
+  Lemma for_map_eval h σc x₁ expr tmp₁ source σ₁ σ₂ d:
+    x₁ <> tmp₁ ->
+    ~ In x₁ (nnrs_imp_expr_free_vars expr) ->
+    ~ In x₁ (domain σ₁) ->
+    nnrs_imp_stmt_eval h σc
+                       (NNRSimpFor tmp₁ source
+                                   (NNRSimpAssign x₁
+                                                  (NNRSimpBinop
+                                                     OpBagUnion
+                                                     (NNRSimpVar x₁)
+                                                     expr))) (σ₁++(x₁,Some (dcoll d))::σ₂) =
+    match nnrs_imp_expr_eval h σc (σ₁++(x₁,Some (dcoll d))::σ₂) source with
+    | Some (dcoll s) =>
+      lift (fun dd => (σ₁++(x₁,Some (dcoll (d++concat dd)))::σ₂))
+           (lift_map (fun dd =>
+                        match
+                          nnrs_imp_expr_eval h σc ((tmp₁, Some dd)::σ₁++σ₂) expr with
+                        | Some (dcoll l) => Some l
+                        | _ => None
+                        end
+                     ) s)
+    | _ => None
+    end.
+  Proof.
+    simpl; intros neq nin1 nin2.
+    match_option.
+    destruct d0; trivial.
+    clear source eqq.
+    revert d.
+    induction l; simpl; intros d.
+    - rewrite app_nil_r; trivial.
+    - unfold var in *.
+      destruct (x₁ == tmp₁); try congruence.
+      destruct (string_dec x₁ tmp₁); try congruence.
+      rewrite lookup_app.
+      rewrite lookup_nin_none by trivial.
+      unfold id; simpl.
+      destruct (x₁ == x₁); try congruence.
+      simpl.
+      generalize (nnrs_imp_expr_eval_unused h σc ((tmp₁, Some a) :: σ₁) σ₂ expr x₁ (Some (dcoll d))); simpl; intros HH; unfold var in *.
+      rewrite HH by tauto; clear HH.
+      case_eq (nnrs_imp_expr_eval h σc ((tmp₁, Some a) :: σ₁ ++ σ₂) expr)
+      ; simpl; trivial; intros d' eqq.
+      destruct d'; simpl; trivial.
+      rewrite lookup_app.
+      rewrite lookup_nin_none by trivial.
+      rewrite update_app_nin by trivial.
+      simpl.
+      destruct (string_dec x₁ x₁); try congruence.
+      rewrite IHl.
+      unfold lift.
+      match_destr; simpl.
+      unfold bunion.
+      rewrite app_ass.
+      trivial.
+  Qed.
+
+    Ltac disect_tac H stac
+    := 
+      unfold var in *
+      ; cut_to H; unfold domain in *; [ | solve[stac]..]
+      ; unfold lift2P in H
+      ; (repeat match_option_in H; try contradiction).
+
+  Ltac pcong
+    := solve[repeat (match goal with
+                     | [H: _ = _ |- _ ] => rewrite H in *; clear H
+                     end; try tauto)].
+
+  Ltac fuse_t stac
+    := repeat progress (
+                repeat rewrite in_app_iff in *
+                ; repeat
+                    match goal with
+                    | [H : ~ (_ \/ _ ) |- _ ] => apply not_or in H
+                    | [H : (_ \/ _ ) -> False |- _ ] => apply not_or in H
+                    | [H: _ /\ _ |- _ ] => destruct H
+                    | [ H : _ * _ |- _ ] => destruct H
+                    | [H: _::_ = _::_ |- _ ] => invcs H
+                    | [ H: domain (_ ++ _) = domain _ |- _ ] =>
+                      rewrite domain_app in H
+                      ; unfold domain in H
+                      ; symmetry in H; apply map_app_break in H
+                      ; destruct H as [? [?[?[??]]]]; subst; simpl in *
+                    | [ H: map (_ ++ _) = map _ |- _ ] =>
+                      rewrite map_app in H
+                      ; symmetry in H; apply map_app_break in H
+                      ; destruct H as [? [?[?[??]]]]; subst; simpl in *
+                    | [ H: _ :: _ = map _ ?x |- _ ] =>
+                      destruct x; try discriminate; simpl in H; invcs H
+                    | [ H: _ :: _ = domain ?x |- _ ] =>
+                      destruct x; try discriminate; simpl in H; invcs H
+                    | [H : ~ In _ (remove _ _ _) |- _ ] =>
+                      apply not_in_remove_impl_not_in in H; [| congruence]
+                    | [H : ?x ++ _ = ?y ++ _ |- _ ] =>
+                      let HH := fresh in
+                      assert (HH:domain y = domain x) by
+                          (unfold domain in *;
+                           try (intuition congruence)
+                           ; pcong)
+                      ; apply app_inv_head_domain in H;[clear HH|apply HH]
+
+                    | [H : nnrs_imp_stmt_eval _ _ _ ?p1 = ?p2 |- _ ] =>
+                          apply nnrs_imp_stmt_eval_domain_stack in H
+
+                    | [ H: forall a b c, _ -> ?x1 :: ?dd :: ?x2 = _ ++ _ :: _ -> _ |- _] =>
+                      specialize (H (x1::nil) (snd dd) x2); simpl in H
+                      ; match dd with
+                        | (_,_) => idtac
+                        | _ => destruct dd
+                        end
+                      ; simpl in *
+                      ; cut_to H; [ | eauto 3 | reflexivity]
+                    end
+                ; simpl in *; trivial; intros; try subst; try contradiction; try solve [congruence | f_equal; congruence]).
+
+    Ltac fuse_tt := fuse_t ltac:(try tauto; try congruence).
+
+  Lemma for_for_fuse_eq x₁ tmp₁ source expr tmp₂ expr₂ tmp₃ body rest :
+    x₁ <> tmp₁ ->
+    x₁ <> tmp₂ ->
+    tmp₂ <> tmp₁ ->
+    ~ In x₁ (nnrs_imp_expr_free_vars expr) ->
+    ~ In x₁ (nnrs_imp_expr_free_vars source) ->
+    ~ In tmp₂ (nnrs_imp_expr_free_vars source) ->
+    ~ In tmp₂ (nnrs_imp_expr_free_vars expr) ->
+    ~ In tmp₁ (nnrs_imp_stmt_free_vars body) ->
+    ~ In x₁ (nnrs_imp_stmt_free_vars body) ->
+    ~ In x₁ (nnrs_imp_stmt_free_vars rest) ->
+    liftP (fun e => ~ In x₁ (nnrs_imp_expr_free_vars e)) expr₂ ->
+    disjoint (nnrs_imp_stmt_maybewritten_vars body) (nnrs_imp_expr_free_vars expr) ->
+    NNRSimpLet x₁ (Some (NNRSimpConst (dcoll nil)))
+                   (NNRSimpSeq
+                      (NNRSimpFor tmp₁ source
+                                  (NNRSimpAssign x₁
+                                              (NNRSimpBinop
+                                                 OpBagUnion
+                                                 (NNRSimpVar x₁)
+                                                 (NNRSimpUnop OpBag expr))))
+                      (NNRSimpLet tmp₂ expr₂
+                                  (NNRSimpSeq
+                                     (NNRSimpFor tmp₃ (NNRSimpVar x₁)
+                                                 body
+                                     )
+                                     rest)))
+                   ≡ˢ
+                   (NNRSimpLet tmp₂ expr₂
+                               (NNRSimpSeq
+                                  (NNRSimpFor tmp₁ source
+                                              (NNRSimpLet tmp₃ (Some expr) body))
+                                  rest)).
+  Proof.
+    Ltac match_in_eq_t
+      := match goal with
+         | [ |- match ?x with | Some _ => _ | None => _ end
+                = match ?y with | Some _ => _ | None => _ end] =>
+           let eqqq := fresh "eqqq" in
+           cut (x=y); [intros eqqq; rewrite eqqq; trivial | ]
+         end.
+
+      red; intros neq1 neq2 neq3 nin1 nin2 nin3 nin4 nin5 nin6 nin7 nin8 disj1; intros; simpl.
+      generalize (nnrs_imp_expr_eval_unused h σc nil σ source)
+      ; simpl; intros HH.
+      repeat rewrite HH by tauto.
+      generalize (for_map_eval h σc x₁ (NNRSimpUnop OpBag expr) tmp₁ source nil σ []); simpl; intros HH2.
+      rewrite HH in HH2 by tauto.
+      rewrite HH2 by tauto; clear HH2.
+      unfold var in *.
+      destruct (x₁ == tmp₁); try congruence; clear c.
+      destruct (x₁ == tmp₂); try congruence; clear c.
+      case_eq (nnrs_imp_expr_eval h σc σ source)
+      ; simpl; [intros ? eqq | intros eqq].
+      2: { idtac.
+           destruct expr₂; simpl; trivial.
+           destruct (nnrs_imp_expr_eval h σc σ n); simpl; trivial.
+           rewrite HH by tauto.
+           rewrite eqq; simpl; trivial.
+           }
+         
+     destruct expr₂; simpl.
+     - transitivity (olift
+    (fun init : option data =>
+     match
+       olift (nnrs_imp_stmt_eval h σc rest)
+         match nnrs_imp_expr_eval h σc σ source with
+         | Some (dcoll c1) =>
+             (fix for_fun (dl : list data) (σ₁ : list (string * option data)) {struct dl} :
+                option (list (string * option data)) :=
+                match dl with
+                | [] => Some σ₁
+                | d1 :: dl' =>
+                    match
+                      olift
+                        (fun init0 : option data =>
+                         match
+                           nnrs_imp_stmt_eval h σc body ((tmp₃, init0) :: (tmp₁, Some d1) :: σ₁)
+                         with
+                         | Some (_ :: σ') => Some σ'
+                         | _ => None
+                         end) (lift Some (nnrs_imp_expr_eval h σc ((tmp₁, Some d1) :: σ₁) expr))
+                    with
+                    | Some (_ :: σ₂) => for_fun dl' σ₂
+                    | _ => None
+                    end
+                end) c1 ((tmp₂, init) :: σ)
+         | _ => None
+         end
+     with
+     | Some (_ :: σ') => Some σ'
+     | _ => None
+     end) (lift Some (nnrs_imp_expr_eval h σc σ n))).
+             2: { idtac.
+                  destruct (lift Some (nnrs_imp_expr_eval h σc σ n)); simpl; trivial.
+                  match_in_eq_t.
+                  f_equal.
+                  rewrite HH by tauto.
+                  rewrite eqq; trivial.
+                  }
+         rewrite eqq.
+         destruct d; simpl
+         ; try solve [unfold olift; match_destr].
+         repeat rewrite olift_lift.
+         simpl.
+         destruct (x₁ == x₁); [| congruence].
+         unfold id; simpl.
+         (* remove unneeded x₁ from n evaluation *)
+         transitivity (
+             match
+               olift
+                 (fun x : list (list data) =>
+                    olift
+                      (fun init : option data =>
+                         match
+                           olift (nnrs_imp_stmt_eval h σc rest)
+                                 ((fix for_fun (dl : list data) (σ₁ : list (string * option data)) {struct dl} :
+                                     option (list (string * option data)) :=
+                                     match dl with
+                                     | [] => Some σ₁
+                                     | d :: dl' =>
+                                       match nnrs_imp_stmt_eval h σc body ((tmp₃, Some d) :: σ₁) with
+                                       | Some (_ :: σ₂) => for_fun dl' σ₂
+                                       | _ => None
+                                       end
+                                     end) (concat x) ((tmp₂, init) :: (x₁, Some (dcoll (concat x))) :: σ))
+                         with
+                         | Some (_ :: σ') => Some σ'
+                         | _ => None
+                         end) (lift Some (nnrs_imp_expr_eval h σc  σ n)))
+                 (lift_map
+                    (fun dd : data =>
+                       match
+                         olift (fun d : data => Some (dcoll [d]))
+                               (nnrs_imp_expr_eval h σc ((tmp₁, Some dd) :: σ) expr)
+                       with
+                       | Some (dcoll l0) => Some l0
+                       | _ => None
+                       end) l)
+             with
+             | Some (_ :: σ') => Some σ'
+             | _ => None
+             end).
+         {
+           match_in_eq_t.
+           apply olift_ext; intros.
+           generalize (nnrs_imp_expr_eval_unused h σc nil σ n)
+           ; simpl; intros HH2.
+           repeat rewrite HH2 by tauto.
+           trivial.
+         }
+         rewrite olift_commute.
+         case_eq (nnrs_imp_expr_eval h σc σ n); simpl; trivial
+         ; intros ? eqq1.
+         replace (lift_map
+         (fun dd : data =>
+          match
+            olift (fun d0 : data => Some (dcoll [d0]))
+              (nnrs_imp_expr_eval h σc ((tmp₁, Some dd) :: σ) expr)
+          with
+          | Some (dcoll l0) => Some l0
+          | _ => None
+          end) l) with
+             (lift_map
+         (fun dd : data =>
+            lift (fun d0 : data => [d0])
+                 (nnrs_imp_expr_eval h σc ((tmp₁, Some dd) :: σ) expr)) l).
+         2: { idtac.
+              apply lift_map_ext; intros.
+              destruct ((nnrs_imp_expr_eval h σc ((tmp₁, Some x) :: σ) expr)); simpl; trivial.
+              }
+            rewrite lift_map_lift.
+              rewrite olift_lift.
+              (* simplify the concat *)
+              transitivity (match
+    olift
+      (fun x : list data =>
+       match
+         olift (nnrs_imp_stmt_eval h σc rest)
+           ((fix for_fun (dl : list data) (σ₁ : list (string * option data)) {struct dl} :
+               option (list (string * option data)) :=
+               match dl with
+               | [] => Some σ₁
+               | d0 :: dl' =>
+                   match nnrs_imp_stmt_eval h σc body ((tmp₃, Some d0) :: σ₁) with
+                   | Some (_ :: σ₂) => for_fun dl' σ₂
+                   | _ => None
+                   end
+               end) x
+              ((tmp₂, Some d)
+               :: (x₁, Some (dcoll x)) :: σ))
+       with
+       | Some (_ :: σ') => Some σ'
+       | _ => None
+       end) (lift_map (fun x : data => nnrs_imp_expr_eval h σc ((tmp₁, Some x) :: σ) expr) l)
+  with
+  | Some (_ :: σ') => Some σ'
+  | _ => None
+                             end).
+              {
+                match_in_eq_t.
+                apply olift_ext; intros.
+                match_in_eq_t.
+                f_equal.
+                rewrite <- flat_map_concat_map, flat_map_singleton; trivial.
+              }
+
+              transitivity (match
+    olift
+      (fun x : list data =>
+       match
+         olift (nnrs_imp_stmt_eval h σc rest)
+               (lift (fun σ =>
+                        match σ with
+                        | xx::σ' => (xx::(x₁, Some (dcoll x))::σ')
+                        | _ => σ
+                        end)
+                  ((fix for_fun (dl : list data) (σ₁ : list (string * option data)) {struct dl} :
+               option (list (string * option data)) :=
+               match dl with
+               | [] => Some σ₁
+               | d0 :: dl' =>
+                   match nnrs_imp_stmt_eval h σc body ((tmp₃, Some d0) :: σ₁) with
+                   | Some (_ :: σ₂) => for_fun dl' σ₂
+                   | _ => None
+                   end
+               end) x ((tmp₂, Some d):: σ)))
+       with
+       | Some (_ :: σ') => Some σ'
+       | _ => None
+       end) (lift_map (fun x : data => nnrs_imp_expr_eval h σc ((tmp₁, Some x) :: σ) expr) l)
+  with
+  | Some (_ :: σ') => Some σ'
+  | _ => None
+                             end).
+              {
+                match_in_eq_t.
+                apply olift_ext; intros.
+                match_in_eq_t.
+                f_equal.
+                clear HH eqq eqq1 H.
+                clear dn_σ.
+                revert σ.
+                generalize (dcoll a).
+                generalize (Some d).
+                induction a; simpl; trivial; intros o dd σ.
+                generalize (nnrs_imp_stmt_eval_unused h σc ((tmp₃, Some a)::(tmp₂, o)::nil) σ body x₁ (Some dd)); simpl; intros HH1.
+                cut_to HH1; [| tauto..].
+                unfold lift2P in HH1.
+                unfold var in *.
+                repeat match_option_in HH1
+                ; fuse_tt.
+                specialize (HH1 ((s, o2) :: (s0, o3)::nil) o4 p0).
+                cut_to HH1; simpl; try tauto.
+                fuse_tt.
+              }
+
+              transitivity (match
+    olift
+      (fun x : list data =>
+       match
+         olift (fun σ => (olift
+              (fun σ0 : list (string * option data) =>
+               match σ0 with
+               | [] => None
+               | xx :: σ' => Some (xx :: (x₁, Some (dcoll x)) :: σ')
+               end) (nnrs_imp_stmt_eval h σc rest σ)))
+              ((fix for_fun (dl : list data) (σ₁ : list (string * option data)) {struct dl} :
+                  option (list (string * option data)) :=
+                  match dl with
+                  | [] => Some σ₁
+                  | d0 :: dl' =>
+                      match nnrs_imp_stmt_eval h σc body ((tmp₃, Some d0) :: σ₁) with
+                      | Some (_ :: σ₂) => for_fun dl' σ₂
+                      | _ => None
+                      end
+                  end) x ((tmp₂, Some d) :: σ))
+       with
+       | Some (_ :: σ') => Some σ'
+       | _ => None
+       end) (lift_map (fun x : data => nnrs_imp_expr_eval h σc ((tmp₁, Some x) :: σ) expr) l)
+  with
+  | Some (_ :: σ') => Some σ'
+  | _ => None
+                             end ).
+              {
+                match_in_eq_t.
+                apply olift_ext; intros.
+                match_in_eq_t.
+                rewrite olift_lift.
+                apply olift_ext; intros.
+                assert (domain ((tmp₂, Some d) :: σ) = domain a0).
+                {
+                  revert H0; clear.
+                  generalize ((tmp₂, Some d)).
+                  revert σ a0.
+                  induction a; simpl; intros.
+                  + invcs H0; simpl; trivial.
+                  + match_option_in H0.
+                    match_destr_in H0.
+                    fuse_tt.
+                    specialize (IHa _ _ _ H0).
+                    simpl in *.
+                    congruence.
+                }
+                simpl in H1.
+                destruct a0; try discriminate.
+                generalize (nnrs_imp_stmt_eval_unused h σc (p::nil) a0 rest x₁ (Some (dcoll a))); simpl; intros HH1.
+                cut_to HH1; [| tauto..].
+                unfold lift2P in HH1.
+                unfold var in *.
+                repeat match_option_in HH1
+                ; fuse_tt.
+              }
+              transitivity (match
+    olift
+      (fun x : list data =>
+           (olift
+              (fun σ0 : list (string * option data) =>
+                 match σ0 with
+                 | [] => None
+                 | xx :: σ' => Some ((x₁, Some (dcoll x)) :: σ')
+                 end)
+         (olift (nnrs_imp_stmt_eval h σc rest)
+              ((fix for_fun (dl : list data) (σ₁ : list (string * option data)) {struct dl} :
+                  option (list (string * option data)) :=
+                  match dl with
+                  | [] => Some σ₁
+                  | d0 :: dl' =>
+                      match nnrs_imp_stmt_eval h σc body ((tmp₃, Some d0) :: σ₁) with
+                      | Some (_ :: σ₂) => for_fun dl' σ₂
+                      | _ => None
+                      end
+                  end) x ((tmp₂, Some d) :: σ))))
+) (lift_map (fun x : data => nnrs_imp_expr_eval h σc ((tmp₁, Some x) :: σ) expr) l)
+  with
+  | Some (_ :: σ') => Some σ'
+  | _ => None
+                             end).
+              {
+                match_in_eq_t.
+                apply olift_ext; intros.
+                destruct (((fix for_fun (dl : list data) (σ₁ : list (string * option data)) {struct dl} :
+          option (list (string * option data)) :=
+          match dl with
+          | [] => Some σ₁
+          | d0 :: dl' =>
+              match nnrs_imp_stmt_eval h σc body ((tmp₃, Some d0) :: σ₁) with
+              | Some (_ :: σ₂) => for_fun dl' σ₂
+              | _ => None
+              end
+          end) a ((tmp₂, Some d) :: σ))); simpl; trivial.
+                destruct (nnrs_imp_stmt_eval h σc rest l0); simpl; trivial.
+                destruct p; simpl; trivial.
+              }
+              (* finally we can get rid of the extra x₁ *)
+              transitivity (match
+                               olift
+                                 (fun x : list data =>
+                                    (olift (nnrs_imp_stmt_eval h σc rest)
+                                           ((fix for_fun (dl : list data) (σ₁ : list (string * option data)) {struct dl} :
+                                               option (list (string * option data)) :=
+                match dl with
+                | [] => Some σ₁
+                | d0 :: dl' =>
+                    match nnrs_imp_stmt_eval h σc body ((tmp₃, Some d0) :: σ₁) with
+                    | Some (_ :: σ₂) => for_fun dl' σ₂
+                    | _ => None
+                    end
+                end) x ((tmp₂, Some d) :: σ))))
+      (lift_map (fun x : data => nnrs_imp_expr_eval h σc ((tmp₁, Some x) :: σ) expr) l)
+  with
+  | Some (_ :: σ') => Some σ'
+  | _ => None
+                             end).
+              {
+                destruct ((lift_map (fun x : data => nnrs_imp_expr_eval h σc ((tmp₁, Some x) :: σ) expr) l)); simpl; trivial.
+                destruct ((olift (nnrs_imp_stmt_eval h σc rest)
+         ((fix for_fun (dl : list data) (σ₁ : list (string * option data)) {struct dl} :
+             option (list (string * option data)) :=
+             match dl with
+             | [] => Some σ₁
+             | d0 :: dl' =>
+                 match nnrs_imp_stmt_eval h σc body ((tmp₃, Some d0) :: σ₁) with
+                 | Some (_ :: σ₂) => for_fun dl' σ₂
+                 | _ => None
+                 end
+             end) l0 ((tmp₂, Some d) :: σ)))); simpl; trivial.
+                destruct p; simpl; trivial.
+              }
+
+              (* swap the olifts *)
+              transitivity (match
+       olift (nnrs_imp_stmt_eval h σc rest)
+             (olift
+                (fun x : list data =>
+         ((fix for_fun (dl : list data) (σ₁ : list (string * option data)) {struct dl} :
+             option (list (string * option data)) :=
+             match dl with
+             | [] => Some σ₁
+             | d0 :: dl' =>
+                 match nnrs_imp_stmt_eval h σc body ((tmp₃, Some d0) :: σ₁) with
+                 | Some (_ :: σ₂) => for_fun dl' σ₂
+                 | _ => None
+                 end
+             end) x ((tmp₂, Some d) :: σ)))
+      (lift_map (fun x : data => nnrs_imp_expr_eval h σc ((tmp₁, Some x) :: σ) expr) l))
+  with
+  | Some (_ :: σ') => Some σ'
+  | _ => None
+  end ).
+              {
+                match_in_eq_t.
+                destruct ((lift_map (fun x : data => nnrs_imp_expr_eval h σc ((tmp₁, Some x) :: σ) expr) l)); simpl; trivial.
+              }
+
+              (* now, let's work on geting rid of the tmp₁ on the other side *)
+              transitivity (match
+    olift (nnrs_imp_stmt_eval h σc rest)
+      ((fix for_fun (dl : list data) (σ₁ : list (string * option data)) {struct dl} :
+          option (list (string * option data)) :=
+          match dl with
+          | [] => Some σ₁
+          | d1 :: dl' =>
+              match
+                olift
+                  (fun init0 : option data =>
+                   match
+                     nnrs_imp_stmt_eval h σc body ((tmp₃, init0) :: σ₁)
+                   with
+                   | Some (_ :: σ') => Some ( (tmp₁, Some d1)::σ')
+                   | _ => None
+                   end) (lift Some (nnrs_imp_expr_eval h σc ((tmp₁, Some d1) :: σ₁) expr))
+              with
+              | Some (_ :: σ₂) => for_fun dl' σ₂
+              | _ => None
+              end
+          end) l ((tmp₂, Some d) :: σ))
+  with
+  | Some (_ :: σ') => Some σ'
+  | _ => None
+                             end).
+              2: { idtac.
+                   match_in_eq_t.
+                   f_equal.
+                   generalize (((tmp₂, Some d) :: σ)).
+                   clear eqq.
+                   induction l; simpl; trivial; intros.
+                   destruct ((lift Some (nnrs_imp_expr_eval h σc ((tmp₁, Some a) :: l0) expr))); simpl; trivial.
+                   generalize (nnrs_imp_stmt_eval_unused h σc ((tmp₃, o)::nil) l0 body tmp₁ (Some a)); simpl; intros HH1.
+                cut_to HH1; [| tauto..].
+                unfold lift2P in HH1.
+                unfold var in *.
+                repeat match_option_in HH1
+                ; fuse_tt.
+                   }
+
+                 (* now that we have moved out the tmp₁, eliminate it *)
+                 (* also simplify the lift Some *)
+                 transitivity (   match
+    olift (nnrs_imp_stmt_eval h σc rest)
+      ((fix for_fun (dl : list data) (σ₁ : list (string * option data)) {struct dl} :
+          option (list (string * option data)) :=
+          match dl with
+          | [] => Some σ₁
+          | d1 :: dl' =>
+              match
+                olift
+                  (fun init0 : data =>
+                   nnrs_imp_stmt_eval h σc body ((tmp₃, Some init0) :: σ₁) 
+                   ) (nnrs_imp_expr_eval h σc ((tmp₁, Some d1) :: σ₁) expr)
+              with
+              | Some (_ :: σ₂) => for_fun dl' σ₂
+              | _ => None
+              end
+          end) l ((tmp₂, Some d) :: σ))
+  with
+  | Some (_ :: σ') => Some σ'
+  | _ => None
+  end).
+                   2: { idtac.
+                        match_in_eq_t.
+                        f_equal.
+                        clear.
+                        generalize ((tmp₂, Some d) :: σ).
+                        induction l; simpl; intros; trivial.
+                        destruct ((nnrs_imp_expr_eval h σc ((tmp₁, Some a) :: l0) expr)); simpl; trivial.
+                        destruct (nnrs_imp_stmt_eval h σc body ((tmp₃, Some d0) :: l0) ); simpl; trivial.
+                        destruct p; simpl; trivial.
+                        }
+                      match_in_eq_t.
+                      f_equal.
+                      clear HH eqq e eqq1.
+                      generalize (Some d); clear d.
+                      clear dn_σ.
+                      revert σ.
+                      induction l; simpl; trivial; intros σ o.
+                      generalize (nnrs_imp_expr_eval_unused h σc ((tmp₁, Some a)::nil) σ expr)
+                      ; simpl; intros HH1.
+                      repeat rewrite HH1 by tauto; clear HH1.
+                      unfold var in *.
+                      destruct (nnrs_imp_expr_eval h σc ((tmp₁, Some a) :: σ) expr)
+                      ; simpl; trivial.
+                      rewrite olift_lift.
+                      (* the body evaluation is independent, so we can pull it out *)
+                      transitivity (
+     match nnrs_imp_stmt_eval h σc body ((tmp₃, Some d) :: (tmp₂, o) :: σ) with
+     | Some (_ :: σ₂) =>
+       olift (fun x : list data =>
+         (fix for_fun (dl : list data) (σ₁ : list (string * option data)) {struct dl} :
+            option (list (string * option data)) :=
+            match dl with
+            | [] => Some σ₁
+            | d0 :: dl' =>
+                match nnrs_imp_stmt_eval h σc body ((tmp₃, Some d0) :: σ₁) with
+                | Some (_ :: σ₂0) => for_fun dl' σ₂0
+                | _ => None
+                end
+            end) x σ₂)
+             (lift_map (fun x : data => nnrs_imp_expr_eval h σc ((tmp₁, Some x) :: σ) expr) l)
+     | _ => None
+     end).
+                      {
+                        clear.
+                        destruct (nnrs_imp_stmt_eval h σc body ((tmp₃, Some d) :: (tmp₂, o) :: σ))
+                        ; destruct ((lift_map (fun x : data => nnrs_imp_expr_eval h σc ((tmp₁, Some x) :: σ) expr) l)); simpl; trivial.
+                        match_destr.
+                      }
+                      match_option.
+                      generalize (nnrs_imp_stmt_eval_domain_stack eqq)
+                      ; simpl ; intros eqq1.
+                      destruct p; simpl in *; try discriminate.
+                      destruct p.
+                      invcs eqq1.
+                      destruct p0; simpl in *; try discriminate.
+                      destruct p.
+                      invcs H1.
+                      rewrite <- IHl.
+                      f_equal.
+                      apply lift_map_ext; intros.
+                      apply nnrs_imp_expr_eval_same.
+                      red; simpl; intros dd inn.
+                      destruct (string_eqdec dd tmp₁); simpl; trivial.
+                      apply (nnrs_imp_stmt_eval_lookup_preserves_unwritten
+                                    ((s, Some d) :: (s0, o)::nil)
+                                    ((s, o0) :: (s0, o1)::nil) _ _ eqq (eq_refl _))
+                      ; simpl.
+                      right.
+                      intros inn2.
+                      apply (disj1 dd); trivial.
+                        - destruct d; simpl; trivial.
+         repeat rewrite olift_lift.
+         simpl.
+         destruct (x₁ == x₁); [| congruence].
+         unfold id; simpl.
+         replace (lift_map
+         (fun dd : data =>
+          match
+            olift (fun d0 : data => Some (dcoll [d0]))
+              (nnrs_imp_expr_eval h σc ((tmp₁, Some dd) :: σ) expr)
+          with
+          | Some (dcoll l0) => Some l0
+          | _ => None
+          end) l) with
+             (lift_map
+         (fun dd : data =>
+            lift (fun d0 : data => [d0])
+                 (nnrs_imp_expr_eval h σc ((tmp₁, Some dd) :: σ) expr)) l).
+         2: { idtac.
+              apply lift_map_ext; intros.
+              destruct ((nnrs_imp_expr_eval h σc ((tmp₁, Some x) :: σ) expr)); simpl; trivial.
+              }
+            rewrite lift_map_lift.
+              rewrite olift_lift.
+              (* simplify the concat *)
+              transitivity (match
+    olift
+      (fun x : list data =>
+       match
+         olift (nnrs_imp_stmt_eval h σc rest)
+           ((fix for_fun (dl : list data) (σ₁ : list (string * option data)) {struct dl} :
+               option (list (string * option data)) :=
+               match dl with
+               | [] => Some σ₁
+               | d0 :: dl' =>
+                   match nnrs_imp_stmt_eval h σc body ((tmp₃, Some d0) :: σ₁) with
+                   | Some (_ :: σ₂) => for_fun dl' σ₂
+                   | _ => None
+                   end
+               end) x
+              ((tmp₂, None)
+               :: (x₁, Some (dcoll x)) :: σ))
+       with
+       | Some (_ :: σ') => Some σ'
+       | _ => None
+       end) (lift_map (fun x : data => nnrs_imp_expr_eval h σc ((tmp₁, Some x) :: σ) expr) l)
+  with
+  | Some (_ :: σ') => Some σ'
+  | _ => None
+                             end).
+              {
+                match_in_eq_t.
+                apply olift_ext; intros.
+                match_in_eq_t.
+                f_equal.
+                rewrite <- flat_map_concat_map, flat_map_singleton; trivial.
+              }
+
+              transitivity (match
+    olift
+      (fun x : list data =>
+       match
+         olift (nnrs_imp_stmt_eval h σc rest)
+               (lift (fun σ =>
+                        match σ with
+                        | xx::σ' => (xx::(x₁, Some (dcoll x))::σ')
+                        | _ => σ
+                        end)
+                  ((fix for_fun (dl : list data) (σ₁ : list (string * option data)) {struct dl} :
+               option (list (string * option data)) :=
+               match dl with
+               | [] => Some σ₁
+               | d0 :: dl' =>
+                   match nnrs_imp_stmt_eval h σc body ((tmp₃, Some d0) :: σ₁) with
+                   | Some (_ :: σ₂) => for_fun dl' σ₂
+                   | _ => None
+                   end
+               end) x ((tmp₂, None):: σ)))
+       with
+       | Some (_ :: σ') => Some σ'
+       | _ => None
+       end) (lift_map (fun x : data => nnrs_imp_expr_eval h σc ((tmp₁, Some x) :: σ) expr) l)
+  with
+  | Some (_ :: σ') => Some σ'
+  | _ => None
+                             end).
+              {
+                match_in_eq_t.
+                apply olift_ext; intros.
+                match_in_eq_t.
+                f_equal.
+                clear HH eqq H.
+                clear dn_σ.
+                revert σ.
+                generalize (dcoll a).
+                generalize ((@None (@data (@foreign_runtime_data fruntime)))).
+                induction a; simpl; trivial; intros o dd σ.
+                generalize (nnrs_imp_stmt_eval_unused h σc ((tmp₃, Some a)::(tmp₂, o)::nil) σ body x₁ (Some dd)); simpl; intros HH1.
+                cut_to HH1; [| tauto..].
+                unfold lift2P in HH1.
+                unfold var in *.
+                repeat match_option_in HH1
+                ; fuse_tt.
+                specialize (HH1 ((s, o2) :: (s0, o3)::nil) o4 p0).
+                cut_to HH1; simpl; try tauto.
+                fuse_tt.
+              }
+
+              transitivity (match
+    olift
+      (fun x : list data =>
+       match
+         olift (fun σ => (olift
+              (fun σ0 : list (string * option data) =>
+               match σ0 with
+               | [] => None
+               | xx :: σ' => Some (xx :: (x₁, Some (dcoll x)) :: σ')
+               end) (nnrs_imp_stmt_eval h σc rest σ)))
+              ((fix for_fun (dl : list data) (σ₁ : list (string * option data)) {struct dl} :
+                  option (list (string * option data)) :=
+                  match dl with
+                  | [] => Some σ₁
+                  | d0 :: dl' =>
+                      match nnrs_imp_stmt_eval h σc body ((tmp₃, Some d0) :: σ₁) with
+                      | Some (_ :: σ₂) => for_fun dl' σ₂
+                      | _ => None
+                      end
+                  end) x ((tmp₂, None) :: σ))
+       with
+       | Some (_ :: σ') => Some σ'
+       | _ => None
+       end) (lift_map (fun x : data => nnrs_imp_expr_eval h σc ((tmp₁, Some x) :: σ) expr) l)
+  with
+  | Some (_ :: σ') => Some σ'
+  | _ => None
+                             end ).
+              {
+                match_in_eq_t.
+                apply olift_ext; intros.
+                match_in_eq_t.
+                rewrite olift_lift.
+                apply olift_ext; intros.
+                assert (domain ((tmp₂, None) :: σ) = domain a0).
+                {
+                  revert H0; clear.
+                  generalize ((tmp₂, (@None (@data (@foreign_runtime_data fruntime))))).
+                  revert σ a0.
+                  induction a; simpl; intros.
+                  + invcs H0; simpl; trivial.
+                  + match_option_in H0.
+                    match_destr_in H0.
+                    fuse_tt.
+                    specialize (IHa _ _ _ H0).
+                    simpl in *.
+                    congruence.
+                }
+                simpl in H1.
+                destruct a0; try discriminate.
+                generalize (nnrs_imp_stmt_eval_unused h σc (p::nil) a0 rest x₁ (Some (dcoll a))); simpl; intros HH1.
+                cut_to HH1; [| tauto..].
+                unfold lift2P in HH1.
+                unfold var in *.
+                repeat match_option_in HH1
+                ; fuse_tt.
+              }
+              transitivity (match
+    olift
+      (fun x : list data =>
+           (olift
+              (fun σ0 : list (string * option data) =>
+                 match σ0 with
+                 | [] => None
+                 | xx :: σ' => Some ((x₁, Some (dcoll x)) :: σ')
+                 end)
+         (olift (nnrs_imp_stmt_eval h σc rest)
+              ((fix for_fun (dl : list data) (σ₁ : list (string * option data)) {struct dl} :
+                  option (list (string * option data)) :=
+                  match dl with
+                  | [] => Some σ₁
+                  | d0 :: dl' =>
+                      match nnrs_imp_stmt_eval h σc body ((tmp₃, Some d0) :: σ₁) with
+                      | Some (_ :: σ₂) => for_fun dl' σ₂
+                      | _ => None
+                      end
+                  end) x ((tmp₂, None) :: σ))))
+) (lift_map (fun x : data => nnrs_imp_expr_eval h σc ((tmp₁, Some x) :: σ) expr) l)
+  with
+  | Some (_ :: σ') => Some σ'
+  | _ => None
+                             end).
+              {
+                match_in_eq_t.
+                apply olift_ext; intros.
+                destruct (((fix for_fun (dl : list data) (σ₁ : list (string * option data)) {struct dl} :
+          option (list (string * option data)) :=
+          match dl with
+          | [] => Some σ₁
+          | d0 :: dl' =>
+              match nnrs_imp_stmt_eval h σc body ((tmp₃, Some d0) :: σ₁) with
+              | Some (_ :: σ₂) => for_fun dl' σ₂
+              | _ => None
+              end
+          end) a ((tmp₂, None) :: σ))); simpl; trivial.
+                destruct (nnrs_imp_stmt_eval h σc rest l0); simpl; trivial.
+                destruct p; simpl; trivial.
+              }
+              (* finally we can get rid of the extra x₁ *)
+              transitivity (match
+                               olift
+                                 (fun x : list data =>
+                                    (olift (nnrs_imp_stmt_eval h σc rest)
+                                           ((fix for_fun (dl : list data) (σ₁ : list (string * option data)) {struct dl} :
+                                               option (list (string * option data)) :=
+                match dl with
+                | [] => Some σ₁
+                | d0 :: dl' =>
+                    match nnrs_imp_stmt_eval h σc body ((tmp₃, Some d0) :: σ₁) with
+                    | Some (_ :: σ₂) => for_fun dl' σ₂
+                    | _ => None
+                    end
+                end) x ((tmp₂, None) :: σ))))
+      (lift_map (fun x : data => nnrs_imp_expr_eval h σc ((tmp₁, Some x) :: σ) expr) l)
+  with
+  | Some (_ :: σ') => Some σ'
+  | _ => None
+                             end).
+              {
+                destruct ((lift_map (fun x : data => nnrs_imp_expr_eval h σc ((tmp₁, Some x) :: σ) expr) l)); simpl; trivial.
+                destruct ((olift (nnrs_imp_stmt_eval h σc rest)
+         ((fix for_fun (dl : list data) (σ₁ : list (string * option data)) {struct dl} :
+             option (list (string * option data)) :=
+             match dl with
+             | [] => Some σ₁
+             | d0 :: dl' =>
+                 match nnrs_imp_stmt_eval h σc body ((tmp₃, Some d0) :: σ₁) with
+                 | Some (_ :: σ₂) => for_fun dl' σ₂
+                 | _ => None
+                 end
+             end) l0 ((tmp₂, None) :: σ)))); simpl; trivial.
+                destruct p; simpl; trivial.
+              }
+
+              (* swap the olifts *)
+              transitivity (match
+       olift (nnrs_imp_stmt_eval h σc rest)
+             (olift
+                (fun x : list data =>
+         ((fix for_fun (dl : list data) (σ₁ : list (string * option data)) {struct dl} :
+             option (list (string * option data)) :=
+             match dl with
+             | [] => Some σ₁
+             | d0 :: dl' =>
+                 match nnrs_imp_stmt_eval h σc body ((tmp₃, Some d0) :: σ₁) with
+                 | Some (_ :: σ₂) => for_fun dl' σ₂
+                 | _ => None
+                 end
+             end) x ((tmp₂, None) :: σ)))
+      (lift_map (fun x : data => nnrs_imp_expr_eval h σc ((tmp₁, Some x) :: σ) expr) l))
+  with
+  | Some (_ :: σ') => Some σ'
+  | _ => None
+  end ).
+              {
+                match_in_eq_t.
+                destruct ((lift_map (fun x : data => nnrs_imp_expr_eval h σc ((tmp₁, Some x) :: σ) expr) l)); simpl; trivial.
+              }
+
+              (* now, let's work on geting rid of the tmp₁ on the other side *)
+              transitivity (match
+    olift (nnrs_imp_stmt_eval h σc rest)
+      ((fix for_fun (dl : list data) (σ₁ : list (string * option data)) {struct dl} :
+          option (list (string * option data)) :=
+          match dl with
+          | [] => Some σ₁
+          | d1 :: dl' =>
+              match
+                olift
+                  (fun init0 : option data =>
+                   match
+                     nnrs_imp_stmt_eval h σc body ((tmp₃, init0) :: σ₁)
+                   with
+                   | Some (_ :: σ') => Some ( (tmp₁, Some d1)::σ')
+                   | _ => None
+                   end) (lift Some (nnrs_imp_expr_eval h σc ((tmp₁, Some d1) :: σ₁) expr))
+              with
+              | Some (_ :: σ₂) => for_fun dl' σ₂
+              | _ => None
+              end
+          end) l ((tmp₂, None) :: σ))
+  with
+  | Some (_ :: σ') => Some σ'
+  | _ => None
+                             end).
+              2: { idtac.
+                   match_in_eq_t.
+                   f_equal.
+                   generalize (((tmp₂, None) :: σ)).
+                   clear eqq.
+                   induction l; simpl; trivial; intros.
+                   destruct ((lift Some (nnrs_imp_expr_eval h σc ((tmp₁, Some a) :: l0) expr))); simpl; trivial.
+                   generalize (nnrs_imp_stmt_eval_unused h σc ((tmp₃, o)::nil) l0 body tmp₁ (Some a)); simpl; intros HH1.
+                cut_to HH1; [| tauto..].
+                unfold lift2P in HH1.
+                unfold var in *.
+                repeat match_option_in HH1
+                ; fuse_tt.
+                   }
+
+                 (* now that we have moved out the tmp₁, eliminate it *)
+                 (* also simplify the lift Some *)
+                 transitivity (   match
+    olift (nnrs_imp_stmt_eval h σc rest)
+      ((fix for_fun (dl : list data) (σ₁ : list (string * option data)) {struct dl} :
+          option (list (string * option data)) :=
+          match dl with
+          | [] => Some σ₁
+          | d1 :: dl' =>
+              match
+                olift
+                  (fun init0 : data =>
+                   nnrs_imp_stmt_eval h σc body ((tmp₃, Some init0) :: σ₁) 
+                   ) (nnrs_imp_expr_eval h σc ((tmp₁, Some d1) :: σ₁) expr)
+              with
+              | Some (_ :: σ₂) => for_fun dl' σ₂
+              | _ => None
+              end
+          end) l ((tmp₂, None) :: σ))
+  with
+  | Some (_ :: σ') => Some σ'
+  | _ => None
+  end).
+                   2: { idtac.
+                        match_in_eq_t.
+                        f_equal.
+                        clear.
+                        generalize ((tmp₂, None) :: σ).
+                        induction l; simpl; intros; trivial.
+                        destruct ((nnrs_imp_expr_eval h σc ((tmp₁, Some a) :: l0) expr)); simpl; trivial.
+                        destruct (nnrs_imp_stmt_eval h σc body ((tmp₃, Some d) :: l0) ); simpl; trivial.
+                        destruct p; simpl; trivial.
+                        }
+                      match_in_eq_t.
+                      f_equal.
+                      clear HH eqq e.
+                      generalize ((@None (@data (@foreign_runtime_data fruntime)))).
+                      clear dn_σ.
+                      revert σ.
+                      induction l; simpl; trivial; intros σ o.
+                      generalize (nnrs_imp_expr_eval_unused h σc ((tmp₁, Some a)::nil) σ expr)
+                      ; simpl; intros HH1.
+                      repeat rewrite HH1 by tauto; clear HH1.
+                      unfold var in *.
+                      destruct (nnrs_imp_expr_eval h σc ((tmp₁, Some a) :: σ) expr)
+                      ; simpl; trivial.
+                      rewrite olift_lift.
+                      (* the body evaluation is independent, so we can pull it out *)
+                      transitivity (
+     match nnrs_imp_stmt_eval h σc body ((tmp₃, Some d) :: (tmp₂, o) :: σ) with
+     | Some (_ :: σ₂) =>
+       olift (fun x : list data =>
+         (fix for_fun (dl : list data) (σ₁ : list (string * option data)) {struct dl} :
+            option (list (string * option data)) :=
+            match dl with
+            | [] => Some σ₁
+            | d0 :: dl' =>
+                match nnrs_imp_stmt_eval h σc body ((tmp₃, Some d0) :: σ₁) with
+                | Some (_ :: σ₂0) => for_fun dl' σ₂0
+                | _ => None
+                end
+            end) x σ₂)
+             (lift_map (fun x : data => nnrs_imp_expr_eval h σc ((tmp₁, Some x) :: σ) expr) l)
+     | _ => None
+     end).
+                      {
+                        clear.
+                        destruct (nnrs_imp_stmt_eval h σc body ((tmp₃, Some d) :: (tmp₂, o) :: σ))
+                        ; destruct ((lift_map (fun x : data => nnrs_imp_expr_eval h σc ((tmp₁, Some x) :: σ) expr) l)); simpl; trivial.
+                        match_destr.
+                      }
+                      match_option.
+                      generalize (nnrs_imp_stmt_eval_domain_stack eqq)
+                      ; simpl ; intros eqq1.
+                      destruct p; simpl in *; try discriminate.
+                      destruct p.
+                      invcs eqq1.
+                      destruct p0; simpl in *; try discriminate.
+                      destruct p.
+                      invcs H1.
+                      rewrite <- IHl.
+                      f_equal.
+                      apply lift_map_ext; intros.
+                      apply nnrs_imp_expr_eval_same.
+                      red; simpl; intros dd inn.
+                      destruct (string_eqdec dd tmp₁); simpl; trivial.
+                      apply (nnrs_imp_stmt_eval_lookup_preserves_unwritten
+                                    ((s, Some d) :: (s0, o)::nil)
+                                    ((s, o0) :: (s0, o1)::nil) _ _ eqq (eq_refl _))
+                      ; simpl.
+                      right.
+                      intros inn2.
+                      apply (disj1 dd); trivial.
+                      
+    Qed.
+      
 End NNRSimpRewrite.
 
